Finished array progress and preservation

elo-coq/Core.v
@@ -22,9 +22,11 @@ Inductive typ : Set :=
   (* primitive types *)
   | TY_Void
   | TY_Num
+  | TY_Arr : typ -> typ
+  | TY_IArr : typ -> typ
   (* internal types *)
   | TY_Ref : typ -> typ
-  | TY_ImmutRef : typ -> typ
+  | TY_IRef : typ -> typ
   | TY_Fun : typ -> typ -> typ
   .
 
@@ -34,9 +36,13 @@ Inductive tm : Set :=
   (* expressions *)
   | TM_Nil
   | TM_Num : num -> tm
+  | TM_Arr : typ -> num -> tm
+  | TM_ArrNew : typ -> tm -> tm
+  | TM_ArrIdx : tm -> tm -> tm
   | TM_Id : name -> tm
   (* statements *)
   | TM_Asg : tm -> tm -> tm
+  | TM_ArrAsg : tm -> tm -> tm -> tm
   | TM_Call : tm -> tm -> tm
   | TM_Seq : tm -> tm -> tm
   (* definitions *)
@@ -54,6 +60,7 @@ Inductive tm : Set :=
 Inductive value : tm -> Prop :=
   | V_Nil : value TM_Nil
   | V_Num : forall n, value (TM_Num n)
+  | V_Arr : forall T i, value (TM_Arr T i)
   (* internal *)
   | V_Loc : forall i, value (TM_Loc i)
   | V_Fun : forall p P block R, value (TM_Fun p P block R)
@@ -76,23 +83,59 @@ Fixpoint subst (id : name) (x t : tm) : tm :=
   match t with
   | TM_Nil => t
   | TM_Num _ => t
-  | TM_Id id' => if id =? id' then x else t
-  | TM_Asg t' e => TM_Asg ([id := x] t') ([id := x] e)
-  | TM_Call f a => TM_Call ([id := x] f) ([id := x] a)
-  | TM_Seq t1 t2 => TM_Seq ([id := x] t1) ([id := x] t2)
-  | TM_LetVal id' E e t' => TM_LetVal id' E ([id := x] e)
-    (if id =? id' then t' else ([id := x] t'))
-  | TM_LetVar id' E e t' => TM_LetVar id' E ([id := x] e)
-    (if id =? id' then t' else ([id := x] t'))
-  | TM_LetFun id' F f t' => TM_LetFun id' F ([id := x] f)
-    (if id =? id' then t' else [id := x] t')
+  | TM_Arr _ _ => t
+  | TM_ArrNew T e =>
+      TM_ArrNew T ([id := x] e)
+  | TM_ArrIdx arr idx =>
+      TM_ArrIdx ([id := x] arr) ([id := x] idx)
+  | TM_Id id' =>
+      if id =? id' then x else t
+  | TM_Asg t' e =>
+      TM_Asg ([id := x] t') ([id := x] e)
+  | TM_ArrAsg arr idx e =>
+      TM_ArrAsg ([id := x] arr) ([id := x] idx) ([id := x] e)
+  | TM_Call f a =>
+      TM_Call ([id := x] f) ([id := x] a)
+  | TM_Seq t1 t2 =>
+      TM_Seq ([id := x] t1) ([id := x] t2)
+  | TM_LetVal id' E e t' =>
+      TM_LetVal id' E ([id := x] e) (if id =? id' then t' else [id := x] t')
+  | TM_LetVar id' E e t' =>
+      TM_LetVar id' E ([id := x] e) (if id =? id' then t' else [id := x] t')
+  | TM_LetFun id' F f t' => 
+      TM_LetFun id' F ([id := x] f) (if id =? id' then t' else [id := x] t')
   | TM_Loc _ => t
-  | TM_Load t' => TM_Load ([id := x] t')
-  | TM_Fun p P block R => if id =? p then t else TM_Fun p P ([id := x] block) R
+  | TM_Load t' =>
+      TM_Load ([id := x] t')
+  | TM_Fun p P block R =>
+      if id =? p then t else TM_Fun p P ([id := x] block) R
   end
   where "'[' id ':=' x ']' t" := (subst id x t).
 
 Inductive step : mem -> tm -> mem -> tm -> Prop :=
+  (* ArrNew *)
+  | ST_ArrNew1 : forall m m' T e e',
+    m / e --> m' / e' ->
+    m / TM_ArrNew T e --> m' / TM_ArrNew T e'
+
+  | ST_ArrNew : forall m T e,
+    value e ->
+    m / TM_ArrNew T e --> (add m e) / TM_Arr T (length m)
+
+  (* ArrIdx *)
+  | ST_ArrIdx1 : forall m m' arr arr' i,
+    m / arr --> m' / arr' ->
+    m / TM_ArrIdx arr i --> m' / TM_ArrIdx arr' i
+
+  | ST_ArrIdx2 : forall m m' arr i i',
+    value arr ->
+    m / i --> m' / i' ->
+    m / TM_ArrIdx arr i --> m' / TM_ArrIdx arr i'
+
+  | ST_ArrIdx : forall m T i j,
+    m / TM_ArrIdx (TM_Arr T i) (TM_Num j) --> m / (get_tm m i)
+
+  (* Asg *)
   | ST_Asg1 : forall m m' t e e',
     m / e --> m' / e' ->
     m / TM_Asg t e --> m' / TM_Asg t e'
@@ -107,6 +150,29 @@ Inductive step : mem -> tm -> mem -> tm -> Prop :=
     i < length m ->
     m / TM_Asg (TM_Loc i) e --> (set m i e) / TM_Nil
 
+  (* ArrAsg *)
+  | ST_ArrAsg1 : forall m m' arr arr' idx e,
+    m / arr --> m' / arr' ->
+    m / TM_ArrAsg arr idx e --> m' / TM_ArrAsg arr' idx e
+
+  | ST_ArrAsg2 : forall m m' arr idx idx' e,
+    value arr ->
+    m / idx --> m' / idx' ->
+    m / TM_ArrAsg arr idx e --> m' / TM_ArrAsg arr idx' e
+
+  | ST_ArrAsg3 : forall m m' arr idx e e',
+    value arr ->
+    value idx ->
+    m / e --> m' / e' ->
+    m / TM_ArrAsg arr idx e --> m' / TM_ArrAsg arr idx e'
+
+  | ST_ArrAsg : forall m T i idx e,
+    value e ->
+    value idx ->
+    i < length m ->
+    m / TM_ArrAsg (TM_Arr T i) idx e --> (set m i e) / TM_Nil
+
+  (* Call *)
   | ST_Call1 : forall m m' f a a',
     m / a --> m' / a' ->
     m / TM_Call f a --> m' / TM_Call f a'
@@ -120,6 +186,7 @@ Inductive step : mem -> tm -> mem -> tm -> Prop :=
     value a ->
     m / TM_Call (TM_Fun p P block R) a --> m / [p := a] block
 
+  (* Seq *)
   | ST_Seq1 : forall m m' t1 t2 t,
     m / t1 --> m' / t2 ->
     m / TM_Seq t1 t --> m' / TM_Seq t2 t
@@ -127,6 +194,7 @@ Inductive step : mem -> tm -> mem -> tm -> Prop :=
   | ST_Seq : forall m t,
     m / TM_Seq TM_Nil t --> m / t
 
+  (* LerVal *)
   | ST_LetVal1 : forall m m' id E e e' t,
     m / e --> m' / e' ->
     m / TM_LetVal id E e t --> m' / TM_LetVal id E e' t
@@ -135,6 +203,7 @@ Inductive step : mem -> tm -> mem -> tm -> Prop :=
     value e ->
     m / TM_LetVal id E e t --> m / [id := e] t
 
+  (* LetVar *)
   | ST_LetVar1 : forall m m' id E e e' t,
     m / e --> m' / e' ->
     m / TM_LetVar id E e t --> m' / TM_LetVar id E e' t
@@ -143,6 +212,7 @@ Inductive step : mem -> tm -> mem -> tm -> Prop :=
     value e ->
     m / TM_LetVar id E e t --> (add m e) / [id := TM_Loc (length m)] t
 
+  (* LetFun *)
   | ST_LetFun1 : forall m m' id F f f' t,
     m / f --> m' / f' ->
     m / TM_LetFun id F f t --> m' / TM_LetFun id F f' t
@@ -151,6 +221,7 @@ Inductive step : mem -> tm -> mem -> tm -> Prop :=
     value f ->
     m / TM_LetFun id F f t --> m / [id := f] t
 
+  (* Load *)
   | ST_Load1 : forall m m' t t',
     m / t --> m' / t' ->
     m / TM_Load t --> m' / TM_Load t'
@@ -169,9 +240,37 @@ Inductive typeof {mt : mem_typ} : ctx -> tm -> typ -> Prop :=
   | T_Num : forall Gamma n,
     Gamma |-- (TM_Num n) is TY_Num
 
+  | T_Arr : forall Gamma T i,
+    T = get_typ mt i -> (* TODO *)
+    i < length mt ->
+    Gamma |-- (TM_Arr (TY_Arr T) i) is (TY_Arr T)
+
+  | T_IArr : forall Gamma T i,
+    T = get_typ mt i -> (* TODO *)
+    i < length mt ->
+    Gamma |-- (TM_Arr (TY_IArr T) i) is (TY_IArr T)
+
+  | T_ArrNew : forall Gamma e E,
+    Gamma |-- e is E ->
+    Gamma |-- (TM_ArrNew (TY_Arr E) e) is (TY_Arr E)
+
+  | T_IArrNew : forall Gamma e E,
+    Gamma |-- e is E ->
+    Gamma |-- (TM_ArrNew (TY_IArr E) e) is (TY_IArr E)
+
+  | T_ArrIdx : forall Gamma arr idx T,
+    Gamma |-- arr is (TY_Arr T) ->
+    Gamma |-- idx is TY_Num ->
+    Gamma |-- (TM_ArrIdx arr idx) is T
+
+  | T_IArrIdx : forall Gamma arr idx T,
+    Gamma |-- arr is (TY_IArr T) ->
+    Gamma |-- idx is TY_Num ->
+    Gamma |-- (TM_ArrIdx arr idx) is T
+
   | T_Id_Val : forall Gamma id T,
-    lookup Gamma id = Some (TY_ImmutRef T) ->
-    Gamma |-- (TM_Id id) is (TY_ImmutRef T)
+    lookup Gamma id = Some (TY_IRef T) ->
+    Gamma |-- (TM_Id id) is (TY_IRef T)
 
   | T_Id_Var : forall Gamma id T,
     lookup Gamma id = Some (TY_Ref T) ->
@@ -181,6 +280,12 @@ Inductive typeof {mt : mem_typ} : ctx -> tm -> typ -> Prop :=
     Gamma |-- t is (TY_Ref T) ->
     Gamma |-- e is T ->
     Gamma |-- (TM_Asg t e) is TY_Void
+
+  | T_ArrAsg : forall Gamma arr idx e E,
+    Gamma |-- arr is (TY_Arr E) ->
+    Gamma |-- idx is TY_Num ->
+    Gamma |-- e is E ->
+    Gamma |-- (TM_ArrAsg arr idx e) is TY_Void
 
   | T_Call : forall Gamma f a P R,
     Gamma |-- f is (TY_Fun P R) ->
@@ -216,8 +321,8 @@ Inductive typeof {mt : mem_typ} : ctx -> tm -> typ -> Prop :=
     Gamma |-- t is TY_Ref T ->
     Gamma |-- (TM_Load t) is T
 
-  | T_Load_ImmutRef : forall Gamma t T,
-    Gamma |-- t is TY_ImmutRef T ->
+  | T_Load_IRef : forall Gamma t T,
+    Gamma |-- t is TY_IRef T ->
     Gamma |-- (TM_Load t) is T
 
   | T_Fun : forall Gamma p P block R,
@@ -246,18 +351,18 @@ Proof.
   intros * Hstep2;
   inversion Hstep2; subst;
   try solve
-    [ exfalso; eapply value_does_not_step; eauto
-    | congruence
+    [ congruence
     | match goal with
-      | F : _ / TM_Loc _ --> _ / _ |- _ => inversion F
-      | F : _ / TM_Nil   --> _ / _ |- _ => inversion F
+      | Hstep : _ / ?v --> _ / _, Hv : value ?v |- _ =>
+        exfalso; apply (value_does_not_step _ _ _ _ Hv Hstep); auto
+      | F : _ / TM_Nil         --> _ / _ |- _ => inversion F
+      | F : _ / TM_Num _       --> _ / _ |- _ => inversion F
+      | F : _ / TM_Arr _ _     --> _ / _ |- _ => inversion F
+      | F : _ / TM_Fun _ _ _ _ --> _ / _ |- _ => inversion F
+      | F : _ / TM_Loc _       --> _ / _ |- _ => inversion F
       | H : forall x, _ / _ --> _ / x -> _ = x |- _ => erewrite H; eauto
       end
     ].
-  - exfalso; eapply (value_does_not_step _ _ (TM_Fun p P block R));
-    eauto using value.
-  - exfalso; eapply (value_does_not_step _ _ (TM_Fun p P block R));
-    eauto using value.
 Qed.
 
 Theorem deterministic_typing : forall mt Gamma t X Y,
@@ -266,9 +371,9 @@ Theorem deterministic_typing : forall mt Gamma t X Y,
   X = Y.
 Proof.
   assert (forall A B, TY_Ref A = TY_Ref B -> A = B). congruence.
-  assert (forall A B, TY_ImmutRef A = TY_ImmutRef B -> A = B). congruence.
-  assert (iref_neq_ref : forall A B, TY_ImmutRef A <> TY_Ref B). congruence.
-  assert (ref_neq_iref : forall A B, TY_Ref A <> TY_ImmutRef B). congruence.
+  assert (forall A B, TY_IRef A = TY_IRef B -> A = B). congruence.
+  assert (iref_neq_ref : forall A B, TY_IRef A <> TY_Ref B). congruence.
+  assert (ref_neq_iref : forall A B, TY_Ref A <> TY_IRef B). congruence.
 
   intros * HX.
   generalize dependent Y.
@@ -279,9 +384,13 @@ Proof.
     exfalso;
     match C with
     | TY_Ref => eapply ref_neq_iref
-    | TY_ImmutRef => eapply iref_neq_ref
+    | TY_IRef => eapply iref_neq_ref
     end;
     eauto
   end; fail).
+  - apply IHHX1 in H4. congruence.
+  - apply IHHX1 in H4. congruence. 
+  - apply IHHX1 in H4. congruence.
+  - apply IHHX1 in H4. congruence.
   - apply IHHX1 in H4. apply IHHX2 in H6. congruence.
 Qed.
